CaseStudies/ABP/Medium.thy
@@ -52,8 +52,8 @@ lemma tsmed_delayfun: "ora\<noteq>\<epsilon> \<Longrightarrow> tsMed\<cdot>(dela
 
 (* ToDo: basic properties lemmata for medium *)
 
-lemma tsmed_nbot [simp]: "msg\<noteq>\<bottom> \<Longrightarrow> #ora=\<infinity> \<Longrightarrow> tsMed\<cdot>msg \<noteq> \<bottom>"
-  oops
+lemma tsmed_nbot [simp]: "msg\<noteq>\<bottom> \<Longrightarrow> #ora=\<infinity> \<Longrightarrow> tsMed\<cdot>msg\<cdot>ora \<noteq> \<bottom>"
+ by (simp add: tsmed_insert)
 
 text {* If infinite ticks will be sent infinite ticks will be transmitted. *}
 lemma tsmed_tstickcount [simp]: "#ora=\<infinity> \<Longrightarrow> #\<surd>(tsMed\<cdot>msg\<cdot>ora) = #\<surd>msg"
@@ -61,7 +61,7 @@ lemma tsmed_tstickcount [simp]: "#ora=\<infinity> \<Longrightarrow> #\<surd>(tsM
 
 text {* If just infinite ticks will be sent just infinite ticks will be transmitted. *}
 lemma tsmed_inftick [simp]: "#ora=\<infinity> \<Longrightarrow> tsMed\<cdot>tsInfTick\<cdot>ora = tsInfTick"
-  apply (simp add: tsmed_insert tsInfTick_def tsfilter_unfold)
+  apply (simp add: tsmed_insert tsInfTick_def tsfilter_insert)
   by (metis (no_types, lifting)
       Inf'_neq_0 Rep_tstream_inject delayfun_insert insertI1 s2sinftimes sfilter_in
       sinftimes_unfold slen_empty_eq tick_msg tsInfTick.abs_eq tsInfTick.rep_eq
@@ -71,7 +71,14 @@ lemma tsmed_inftick [simp]: "#ora=\<infinity> \<Longrightarrow> tsMed\<cdot>tsIn
 
 text {* Medium without oracle will transmit all messages and ticks. *}
 lemma tsmed_inftrue [simp]: "tsMed\<cdot>msg\<cdot>((\<up>True) \<infinity>) = msg"
-  oops
+  apply(simp add: tsmed_insert)
+  apply (induction msg)
+  apply (simp_all)
+  apply (metis lscons_conv sinftimes_unfold stream.con_rews(2)
+         tsmed_delayfun tsmed_insert up_defined)
+  by (metis lscons_conv sinftimes_unfold slen_sinftimes strict_icycle
+      tsmed_insert tsmed_mlscons_true tsmed_strict(2))
+
 
 text {* Not every message will be transmitted. *}    
 lemma tsmed_tsabs_slen: "#ora=\<infinity> \<Longrightarrow> #(tsAbs\<cdot>(tsMed\<cdot>msg\<cdot>ora)) \<le> #(tsAbs\<cdot>msg)"
@@ -84,12 +91,71 @@ text {* If infinite messages will be sent infinite messages will be transmitted.
 lemma tsmed_tsabs_slen_inf [simp]: assumes "#({True} \<ominus> ora)=\<infinity>" and "#(tsAbs\<cdot>msg)=\<infinity>" 
   shows "#(tsAbs\<cdot>(tsMed\<cdot>msg\<cdot>ora)) = \<infinity>"
   oops
+(*
+lemma szip_collect_inf_h: assumes "#s=\<infinity>" shows  "#(Collect snd \<ominus> s) = \<infinity>" 
+  sorry
+    
+lemma szip_collect_inf: assumes "#ora=\<infinity>" and "#msg=\<infinity>"
+  shows "#(Collect snd \<ominus> szip\<cdot>msg\<cdot>ora) = \<infinity>"
+  by (simp add: assms(1) assms(2) szip_collect_inf_h)
+*)
+    
+lemma tsmed_map: "#ora=\<infinity> \<Longrightarrow> tsMed\<cdot>(tsMap f\<cdot>msg)\<cdot>ora = tsMap f\<cdot>(tsMed\<cdot>msg\<cdot>ora)"
+  apply(induct msg arbitrary: ora, auto)
+  apply (metis tsmap_delayfun tsmed_delayfun tsmed_strict(2))
+  apply(rule_tac x=ora in scases, simp_all)
+  apply(rename_tac y x )
+  apply (case_tac "y=True", simp_all)
+  apply (metis (no_types, lifting) lscons_conv tsmap_mlscons tsmap_nbot tsmed_mlscons_true tsmed_nbot)
+  by (metis lscons_conv tsmap_mlscons tsmap_nbot tsmed_mlscons_false)
 
-lemma tsmed_map: "tsMed\<cdot>(tsMap f\<cdot>msg)\<cdot>ora = tsMap f\<cdot>(tsMed\<cdot>msg\<cdot>ora)"
-  oops
 
 lemma tsmed_tsdom: "#ora=\<infinity> \<Longrightarrow> tsDom\<cdot>(tsMed\<cdot>msg\<cdot>ora) \<subseteq> tsDom\<cdot>msg"
-  oops
+proof(induction msg arbitrary: ora)
+ case adm
+   then show ?case 
+     apply (rule admI)
+     by (simp add: contlub_cfun_arg contlub_cfun_fun lub_eq_Union SUP_subset_mono)
+ next
+   case bottom
+   then show ?case 
+     by simp
+ next
+   case (delayfun msg)
+   then show ?case 
+     by (metis Inf'_neq_0 strict_slen tsdom_delayfun tsmed_delayfun)
+ next
+  case (mlscons msg t)
+  then show ?case 
+  proof -
+    
+  have lscons_conv_for_True: "\<up>True \<bullet> ora= (updis True) && ora"
+    by(simp add:lscons_conv)  
+  hence tsmed_mlscons_true_less_assms: "#ora=\<infinity>  \<Longrightarrow> tsMed\<cdot>(tsMLscons\<cdot>(updis t)\<cdot>msg)\<cdot>(\<up>True \<bullet> ora) =  tsMLscons\<cdot>(updis t)\<cdot>(tsMed\<cdot>msg\<cdot>ora)"
+    using tsmed_mlscons_true by force
+      
+  (* can I user scases somehow here?*)
+  have ora_split: "ora = \<up>(shd ora) \<bullet> srt\<cdot>ora \<and> #(srt\<cdot>ora) = \<infinity>"
+    by (metis Inf'_neq_0 fold_inf inject_lnsuc mlscons.prems slen_empty_eq srt_decrements_length surj_scons)    
+  have tsdom_ora_srt: "tsDom\<cdot>(tsMed\<cdot>msg\<cdot>(srt\<cdot>ora)) \<subseteq> {t} \<union> tsDom\<cdot>msg"
+    by (metis Inf'_neq_0 fold_inf inject_lnsuc mlscons.IH mlscons.prems slen_empty_eq srt_decrements_length sup.coboundedI2)
+      
+  { 
+    assume "({t} \<union> tsDom\<cdot>(tsMed\<cdot>msg\<cdot>(srt\<cdot>ora)) \<subseteq> {t} \<union> tsDom\<cdot>msg) \<noteq>
+            (tsDom\<cdot>(tsMed\<cdot>(tsMLscons\<cdot>(updis t)\<cdot>msg)\<cdot>ora) \<subseteq> tsDom\<cdot>(tsMLscons\<cdot>(updis t)\<cdot>msg))"
+      
+    then have "{t} \<union> tsDom\<cdot>(tsMed\<cdot>msg\<cdot>(srt\<cdot>ora)) \<noteq> tsDom\<cdot>(tsMed\<cdot>(tsMLscons\<cdot>(updis t)\<cdot>msg)\<cdot>ora)"
+      using mlscons.hyps tsdom_mlscons by fastforce    
+    then have "\<up>True \<bullet> srt\<cdot>ora \<noteq> ora"
+      by (metis ora_split lscons_conv mlscons.hyps tsdom_mlscons tsmed_mlscons_true tsmed_nbot)        
+    then have ?thesis 
+     by (metis (full_types) ora_split tsdom_ora_srt lscons_conv mlscons.hyps tsdom_mlscons tsmed_mlscons_false) }
+    
+  then show ?thesis
+    using tsdom_ora_srt by auto
+  qed
+qed
+
 
 (* ----------------------------------------------------------------------- *)
 section {* additional properties *}
